fowl/Has/Isomorphism.v
@@ -1,8 +1,0 @@
-(** Isomorphism, Proof-Irrelevant Equivalence, Bijection *)
-
-From Maniunfold Require Export
-  Init.
-
-Class HasIso (A B : Type) : Type := iso : (A -> B) * (B -> A).
-
-Typeclasses Transparent HasIso.
