fowl/Offers/OneSortedEnumeration.v
@@ -2,17 +2,15 @@
 From Coq Require Import
   NArith.NArith Lists.List.
 From Maniunfold.Has Require Export
-  OneSortedCardinality Isomorphism.
+  OneSortedCardinality.
 From Maniunfold.Is Require Export
   OneSortedFinite Isomorphism.
-From Maniunfold.Offers Require Export
-  IsomorphismMappings.
 
 Local Open Scope N_scope.
 
 Section Context.
 
-Context (A : Type) `{IsFin A}.
+Context (A : Type) `(IsFin A).
 
 Import N.
 
@@ -25,7 +23,7 @@ Definition enum : list A.
 Proof.
   set (ns := map of_nat (seq O (to_nat (card A)))).
   refine (map _ ns).
-  intros n. apply retr. exists n.
+  intros n. apply g. exists n.
   apply violence. Defined.
 
 (** TODO Prove that [enum] is a disjoint cover of [A]:
